\documentclass{article}
\usepackage{amsmath}
\title{Homework 2 - Logic (Spring 2021)}
\author
{
Ryan, Soeyadi
\and rs4163
}


\begin{document}
    \maketitle
    
    \section*{Question 1}
    $\neg p \lor (q \land (r \lor p))$
    \begin{displaymath}
    \begin{array}{|c|c|c|c|c|c|c|}
    
    p & q & r & r \lor p & q \land (r \lor p) & \neg p & \neg p \lor (q \land (r \lor p)) \\
    \hline
    T & T & T & T & T & F & T \\
    T & T & F & T & T & F & T \\
    T & F & T & T & F & F & F \\
    T & F & F & T & F & F & F \\
    F & T & T & T & T & T & T \\
    F & T & F & F & F & T & T \\
    F & F & T & T & F & T & T \\
    F & F & F & F & F & T & T \\
    \end{array}
    \end{displaymath}
    \newpage
    \section*{Question 2}
     This proposition is True since the antecedent is False; there are no two integers that fit the criteria to make it True. Therefore, it does not matter if the right side, the consequence, is True or not.
    \newpage
    \section*{Question 3}
    \begin{enumerate}
    \item $E \implies Q$ \\
    \item $E \lor B$ \\
    \item $\neg Q$ \\
    \item $\neg (E \lor Q)$ \\
    \item $E \land \neg B$ \\
    \item $\neg B \implies E$ \\
    \item $Q \implies \neg B$
    \end{enumerate}
    \newpage
    \section*{Question 4}
    \begin{enumerate}
    \item 
    $E \implies Q  \equiv \neg E \lor Q$\\
    $\neg E \lor Q$ \\
    $\neg (\neg E \lor Q)$ \\
    $E \land \neg Q$ \\
    \item 
    $E \lor B$ \\
    $\neg (E \lor B)$ \\
    $\neg E \land \neg B$ \\
    \item 
    $\neg Q$ \\
    $\neg (\neg Q)$ \\
    $Q$ \\
    \item 
    $\neg (E \lor Q) \equiv \neg E \land \neg Q$ \\
    $\neg(\neg E \land \neg Q)$ \\
    $E \lor Q$ \\
    \item 
    $E \land \neg B$ \\
    $\neg (E \land \neg B)$ \\
    $\neg E \lor B$ \\
    \item 
    $\neg B \implies E \equiv \neg (\neg B) \lor E$ \\
    $B \lor E$ \\
    $\neg(B \lor E)$ \\
    $\neg B \land \neg E$
    \item 
    $Q \implies \neg B \equiv \neg Q \lor \neg B$ \\
    $\neg (\neg Q \lor \neg B)$ \\
    $Q \land B$ \\
    \end{enumerate}
     \newpage
    \section*{Question 5}
    $\neg p \land (p \lor q) \implies q$ \\
    $\neg p \land (p \lor q) \implies q \equiv \neg (\neg p \land (p \lor q)) \lor q$ \\
    $\neg p \land (p \lor q) \implies q \equiv p \lor \neg(p \lor q) \lor q$ \\
    $\neg p \land (p \lor q) \implies q \equiv p \lor (\neg p \land \neg q) \lor q$ \\
    $\neg p \land (p \lor q) \implies q \equiv (p \lor \neg p) \land (p \lor \neg q) \lor q$ \\
    $\neg p \land (p \lor q) \implies q \equiv True \land (p \lor \neg q) \lor q$ \\
    $\neg p \land (p \lor q) \implies q \equiv True \land q \lor (p \lor \neg q)$ \\
    $\neg p \land (p \lor q) \implies q \equiv True \land (q \lor p) \lor (q \lor \neg q)$ \\
    $\neg p \land (p \lor q) \implies q \equiv True \land (q \lor p) \lor True$ \\
    $\neg p \land (p \lor q) \implies q \equiv True \land True$ \\
    $\neg p \land (p \lor q) \implies q \equiv True$ \\
    Therefore, $\neg p \land (p \lor q) \implies q$ is a Tautology
    
    \newpage
    \section*{Question 6}
    \textbf{if not} ((a $<$ b) \textbf{or} even(a)) \textbf{or} (\textbf{not}(a $<$ b) \textbf{and} even(a)) \\
    \indent c $=$ a $-$ b \\
    \textbf{else:}\\
    \indent c = b $-$ a \\\\
    Let $p =$ (a $<$ b)\\
    Let $q =$ even(a)\\\\	
    $\neg(p \lor q) \lor (\neg p \land q)$ \\
    $(\neg p \land \neg q) \lor (\neg p \land q)$ \\
    $\neg p \land (\neg q \lor q)$ \\
    $\neg p \land True$ \\
    $\neg p$

   \end{document}